{
 "cells": [
  {
   "cell_type": "markdown",
   "metadata": {},
   "source": [
    "[From Briggs, Cochran *Calculus: Early Transcendentals*.]"
   ]
  },
  {
   "cell_type": "code",
   "execution_count": null,
   "metadata": {
    "collapsed": true
   },
   "outputs": [],
   "source": []
  },
  {
   "cell_type": "code",
   "execution_count": null,
   "metadata": {
    "collapsed": true
   },
   "outputs": [],
   "source": []
  },
  {
   "cell_type": "markdown",
   "metadata": {},
   "source": [
    "# 3"
   ]
  },
  {
   "cell_type": "markdown",
   "metadata": {},
   "source": [
    "### Constant Rule\n",
    "If $c$ is a real number, then $\\frac{d}{dx}(c) = 0$\n",
    "\n",
    "### Power Rule\n",
    "If $n$ is a postive integer, then $\\frac{d}{dx}(x^{n}) = nx^{n-1}$\n",
    "\n",
    "##### Definitions\n",
    "$f(x) = x^{n} \\implies f(x) - f(a) = x^{n} - a^{n}$\n",
    "\n",
    "$x^{n} - a^{n} = (x - a)(x^{n-1} + x^{n-2}a + ... + xa^{n-2} + a^{n-1})$\n",
    "\n",
    "$\\lim_{x \\rightarrow a} (x^{n-1} + x^{n-2}a + ... + xa^{n-2} + a^{n-1}) = a^{n-1} + a^{n-2} \\cdot a + ... + a \\cdot a^{n-2} + a^{n-1} = na^{n-1}$\n",
    "\n",
    "##### Definition Examples\n",
    "$x^{4} - a^{4} = (x - a)(x^{3} + x^{2}a + xa^{2} + a^{3})$\n",
    "\n",
    "$\\lim_{x \\rightarrow a} (x^{3} + x^{2}a + xa^{2} + a^{3}) = a^{3} + a^{2} \\cdot a + a \\cdot a^{2} = a^{3} + a^{3} + a^{3} = 3n^{3}$\n",
    "\n",
    "##### Proof\n",
    "$$\n",
    "\\begin{align}\n",
    "f'(a) &= \\lim_{x \\rightarrow a} \\frac{f(x) - f(a)}{x - a} \\\\\n",
    "&= \\lim_{x \\rightarrow a} \\frac{x^{n} - a^{n}}{x - a} \\\\\n",
    "&= \\lim_{x \\rightarrow a} \\frac{(x - a)(x^{n-1} + x^{n-2}a + ... + xa^{n-2} + a^{n-1})}{x - a} \\\\\n",
    "&= \\lim_{x \\rightarrow a} (x^{n-1} + x^{n-2}a + ... + xa^{n-2} + a^{n-1}) \\\\\n",
    "&= a^{n-1} + a^{n-2} \\cdot a + ... + a \\cdot a^{n-2} + a^{n-1} \\\\\n",
    "&= na^{a-1}\n",
    "\\end{align}\n",
    "$$"
   ]
  },
  {
   "cell_type": "markdown",
   "metadata": {},
   "source": [
    "### The derivative of $e^{x}$\n",
    "The function $f(x) = e^{x}$ is differentiable for all real numbers $x$ and\n",
    "$$\\frac{d}{dx}(e^{x}) = e^{x}$$\n",
    "\n",
    "##### Proof\n",
    "$$\n",
    "\\begin{align}\n",
    "\\frac{d}{dx}(e^{x}) &= \\lim_{h \\rightarrow 0} \\frac{e^{x + h} - e^{x}}{h} \\\\\n",
    "&= \\lim_{h \\rightarrow 0} \\frac{e^{x} \\cdot e^{h} - e^{x}}{h} \\\\\n",
    "&= \\lim_{h \\rightarrow 0} \\frac{e^{x}(e^{h} - 1)}{h} \\\\ \n",
    "&= e^{x} \\cdot \\lim_{h \\rightarrow 0} \\frac{e^{h} - 1}{h} \\\\\n",
    "&= e^{x} \\cdot 1 = e^{x}\n",
    "\\end{align}\n",
    "$$"
   ]
  },
  {
   "cell_type": "markdown",
   "metadata": {},
   "source": [
    "### Product Rule\n",
    "If $f$ and $g$ are differentiable at $x$, then\n",
    "$$\\frac{d}{dx}[f(x)g(x)] = f'(x)g(x) + f(x)g'(x)$$\n",
    "\n",
    "##### Definitions\n",
    "$Z: -f(x)g(x+h) + f(x)g(x + h) = 0$  \n",
    "\n",
    "$\\lim_{h \\rightarrow 0} f(x) = f(x)$\n",
    "\n",
    "$\\lim_{h \\rightarrow 0} \\frac{f(x + h) - f(x)}{h} = f'(x)$\n",
    "\n",
    "$\\lim_{h \\rightarrow 0} g(x + h) = g(x)$\n",
    "\n",
    "$\\lim_{h \\rightarrow 0} \\frac{g(x + h) - g(x)}{h} = g'(x)$\n",
    "\n",
    "##### Proof\n",
    "$$\n",
    "\\begin{align}\n",
    "\\frac{d}{dx}[f(x)g(x)] &= \\lim_{h \\rightarrow 0} \\frac{f(x + h)g(x + h) - f(x)g(x)}{h} \\\\\n",
    "&= \\lim_{h \\rightarrow 0} \\frac{f(x + h)g(x + h) - f(x)g(x) + Z}{h} \\\\\n",
    "&= \\lim_{h \\rightarrow 0} \\frac{f(x + h)g(x + h) - f(x)g(x) + [-f(x)g(x+h) + f(x)g(x + h)]}{h} \\\\\n",
    "&= \\lim_{h \\rightarrow 0} \\frac{f(x + h)g(x + h) - f(x)g(x+h) + f(x)g(x + h) - f(x)g(x)}{h} \\\\\n",
    "&= \\lim_{h \\rightarrow 0} \\frac{f(x + h)g(x + h) - f(x)g(x+h)}{h} + \\lim_{h \\rightarrow 0} \\frac{f(x)g(x + h) - f(x)g(x)}{h} \\\\\n",
    "&= \\lim_{h \\rightarrow 0} \\bigg[\\frac{f(x + h) - f(x)}{h} \\cdot g(x + h)\\bigg] + \\lim_{h \\rightarrow 0} \\bigg[f(x) \\cdot \\frac{g(x + h) - g(x)}{h} \\bigg] \\\\\n",
    "&= f'(x) \\cdot g(x) + f(x) \\cdot g'(x)\n",
    "\\end{align}\n",
    "$$\n",
    "\n",
    "### Quotient Rule\n",
    "If $f$ and $q$ are differentiable at $x$, then the derivative of $f/g$ at $x$ exists provided $g(x) \\neq 0$ and\n",
    "\n",
    "$$\\frac{d}{dx}\\bigg[\\frac{f(x)}{g(x)}\\bigg] = \\frac{g(x)f'(x) - f(x)g'(x)}{[g(x)]^{2}}$$\n",
    "\n",
    "##### Definitions\n",
    "$q(x) = \\frac{f(x)}{g(x)}$\n",
    "\n",
    "$f(x) = g(x)q(x)$\n",
    "\n",
    "##### Calculation\n",
    "If $\\frac{d}{dx}f/g$ exists,\n",
    "$$\n",
    "\\begin{align}\n",
    "f'(x) &= g'(x)q(x) + g(x)q'(x) \\\\\n",
    "q'(x) &= \\frac{f'(x) - g'(x)q(x)}{g(x)} \\\\\n",
    "q'(x) &= \\frac{f'(x) - g'(x)\\frac{f(x)}{g(x)}}{g(x)} \\\\\n",
    "&= \\frac{g(x) \\Big(f'(x) - g'(x)\\frac{f(x)}{g(x)}\\Big)}{g(x) \\cdot g(x)} \\\\\n",
    "&= \\frac{g(x)f'(x) - f(x)g'(x)}{[g(x)]^{2}}\n",
    "\\end{align}\n",
    "$$\n",
    "\n",
    "##### Definitions\n",
    "Let $F = f/g$ be the quotient of two functions that are differentiable at $x$\n",
    "\n",
    "$Z: -f(x)g(x) + f(x)g(x) = 0$  \n",
    "\n",
    "$\\lim_{h \\rightarrow 0} f(x) = f(x)$\n",
    "\n",
    "$\\lim_{h \\rightarrow 0} \\frac{f(x + h) - f(x)}{h} = f'(x)$\n",
    "\n",
    "$\\lim_{h \\rightarrow 0} g(x) = g(x)$\n",
    "\n",
    "$\\lim_{h \\rightarrow 0} \\frac{g(x) - g(x + h)}{h} = -g'(x)$\n",
    "\n",
    "$\\lim_{h \\rightarrow 0} \\frac{1}{g(x)g(x + h)} = \\frac{1}{[g(x)]^{2}}$\n",
    "\n",
    "##### Proof\n",
    "$$\n",
    "\\begin{align}\n",
    "\\frac{d}{dx}[f(x)g(x)] &= \\lim_{h \\rightarrow 0} \\frac{\\frac{f(x + h)}{g(x + h)} - \\frac{f(x)}{g(x)}}{h} \\\\\n",
    "&= \\lim_{h \\rightarrow 0} \\frac{f(x + h)}{g(x + h) \\cdot h} - \\frac{f(x)}{g(x) \\cdot h} \\\\\n",
    "&= \\lim_{h \\rightarrow 0} \\frac{f(x + h)g(x) - f(x)g(x + h)}{g(x)g(x + h) \\cdot h} \\\\\n",
    "&= \\lim_{h \\rightarrow 0} \\frac{f(x + h)g(x) - f(x)g(x + h) + Z}{g(x)g(x + h) \\cdot h} = \\lim_{h \\rightarrow 0} \\frac{f(x + h)g(x) - f(x)g(x + h) + [-f(x)g(x) + f(x)g(x)]}{g(x)g(x + h) \\cdot h} \\\\\n",
    "&= \\lim_{h \\rightarrow 0} \\frac{f(x + h)g(x) - f(x)g(x) + g(x)f(x) - g(x+h)f(x)}{g(x)g(x + h) \\cdot h} \\\\\n",
    "&= \\lim_{h \\rightarrow 0} \\frac{f(x + h)g(x) - f(x)g(x)}{g(x)g(x + h) \\cdot h} + \\frac{g(x)f(x) - g(x + h)f(x)}{g(x)g(x + h) \\cdot h} \\\\\n",
    "&= \\bigg[\\lim_{h \\rightarrow 0} \\frac{f(x + h) - f(x)}{g(x)g(x + h) \\cdot h} \\cdot g(x) \\bigg] + \\bigg[\\lim_{h \\rightarrow 0} \\frac{g(x) - g(x + h)}{g(x)g(x + h) \\cdot h} \\cdot f(x)\\bigg] \\\\\n",
    "&= \\bigg[\\lim_{h \\rightarrow 0} \\frac{f(x + h) - f(x)}{h} \\cdot g(x) \\cdot \\frac{1}{g(x)g(x + h)} \\bigg] + \\bigg[\\lim_{h \\rightarrow 0} \\frac{g(x) - g(x + h)}{h} \\cdot f(x)  \\cdot \\frac{1}{g(x)g(x + h)} \\bigg] \\\\\n",
    "&= \\bigg[f'(x) \\cdot g(x) \\cdot \\frac{1}{[g(x)]^{2}} \\bigg] + \\bigg[-g'(x) \\cdot f(x)  \\cdot \\frac{1}{[g(x)]^{2}} \\bigg] \\\\\n",
    "&= \\frac{f'(x)g(x) - g'(x)f(x)}{[g(x)]^{2}}\n",
    "\\end{align}\n",
    "$$\n",
    "\n",
    "### The derivative of $e^{kx}$\n",
    "For real numbers $k$, \n",
    "$$\\frac{d}{dx}(e^{kx}) = ke^{kx}$$\n",
    "\n",
    "##### Example\n",
    "$$\n",
    "\\begin{align}\n",
    "\\frac{d}{dx}(e^{2x}) &= \\frac{d}{dx}(e^{x} \\cdot e^{x}) \\\\\n",
    "&= \\frac{d}{dx}(e^{x}) \\cdot e^{x} + e^{x} \\cdot \\frac{d}{dx}(e^{x}) \\\\\n",
    "&= e^{x} \\cdot e^{x} + e^{x} \\cdot e^{x} = 2e^{2x}\n",
    "\\end{align}\n",
    "$$\n",
    "\n",
    "##### Proof by induction for positive integers $k$\n",
    "Base case ($k = 1$)\n",
    "$$\n",
    "\\begin{align}\n",
    "\\frac{d}{dx}e^{kx} &= \\frac{d}{dx}e^{1 \\cdot x} \\\\\n",
    "&= \\frac{d}{dx}e^{x} \\\\\n",
    "&= e^{x}\n",
    "\\end{align}\n",
    "$$\n",
    "\n",
    "Inductive step (inductive hypothesis: assume true for $k = n$)\n",
    "$$\n",
    "\\begin{align}\n",
    "\\frac{d}{dx}e^{nx} = ne^{nx}\n",
    "\\end{align}\n",
    "$$\n",
    "\n",
    "Prove true for $k = n + 1$: $\\frac{d}{dx}e^{(n+1)x} = (n+1)e^{(n+1)x}$\n",
    "\n",
    "$$\n",
    "\\begin{align}\n",
    "\\frac{d}{dx}e^{(n+1)x} &= \\frac{d}{dx}e^{nx + x} \\\\\n",
    "&= \\frac{d}{dx}(e^{nx} \\cdot e^{x}) \\\\\n",
    "&= ne^{nx} \\cdot e^{x} + e^{nx} \\cdot e^{x} \\\\\n",
    "&= e^{x}(ne^{nx} + e^{nx}) \\\\\n",
    "&= e^{x} \\cdot e^{nx}(n + 1) \\\\\n",
    "&= e^{nx+x}(n+1) \\\\\n",
    "&= e^{(n+1)x}(n+1) \\\\\n",
    "&= (n+1)e^{(n+1)x}\n",
    "\\end{align}\n",
    "$$\n",
    "\n",
    "##### Proof by induction for negative integers $k$\n",
    "Base case ($k = -1$)\n",
    "$$\n",
    "\\begin{align}\n",
    "\\frac{d}{dx}e^{kx} &= \\frac{d}{dx}e^{-1 \\cdot x} \\\\\n",
    "&= \\frac{d}{dx}e^{-x} = \\frac{d}{dx}\\bigg(\\frac{1}{e^{x}}\\bigg) \\\\\n",
    "&= \\frac{o \\cdot e^{x} - 1 \\cdot e^{x}}{e^{x} \\cdot e^{x}} = \\frac{-e^{x}}{[e^{x}]^{2}} = \\frac{-1}{e^{x}} = -e^{-x}\n",
    "\\end{align}\n",
    "$$\n",
    "\n",
    "Inductive step (inductive hypothesis: assume true for $k = -n$)\n",
    "$$\n",
    "\\begin{align}\n",
    "\\frac{d}{dx}e^{-nx} = -ne^{-nx}\n",
    "\\end{align}\n",
    "$$\n",
    "\n",
    "Prove true for $k = -n - 1$: $\\frac{d}{dx}e^{(-n - 1)x} = (-n - 1)e^{(-n - 1)x}$\n",
    "\n",
    "$$\n",
    "\\begin{align}\n",
    "\\frac{d}{dx}e^{(-n - 1)x} &= \\frac{d}{dx}e^{-nx - x} \\\\\n",
    "&= \\frac{d}{dx}(e^{-nx} \\cdot e^{-x}) \\\\\n",
    "&= \\frac{d}{dx}\\bigg(\\frac{e^{-nx}}{e^{x}}\\bigg) \\\\\n",
    "&= \\frac{-ne^{-nx} \\cdot e^{x} - e^{-nx} \\cdot e^{x}}{e^{x} \\cdot e^{x}} = \\frac{e^{x}(-ne^{-nx} - e^{-nx})}{e^{x} \\cdot e^{x}} = \\frac{-ne^{-nx} - e^{-nx}}{e^{x}} = \\frac{e^{-nx}(-n - 1)}{e^{x}} \\\\\n",
    "&= e^{-nx} \\cdot e^{-x} (-n - 1) = e^{-nx-x}(-n - 1) = e^{(-n - 1)x}(-n - 1) = (-n - 1)e^{(-n - 1)x} \n",
    "\\end{align}\n",
    "$$"
   ]
  }
 ],
 "metadata": {
  "kernelspec": {
   "display_name": "Python [conda env:math]",
   "language": "python",
   "name": "conda-env-math-py"
  },
  "language_info": {
   "codemirror_mode": {
    "name": "ipython",
    "version": 3
   },
   "file_extension": ".py",
   "mimetype": "text/x-python",
   "name": "python",
   "nbconvert_exporter": "python",
   "pygments_lexer": "ipython3",
   "version": "3.5.2"
  }
 },
 "nbformat": 4,
 "nbformat_minor": 1
}
